Using the appropriate no-arbitrage condition, derive the equation that allows us to pin-down the coefficient $\kappa_{1,d}$ for the Campbell and Shiller approximation in the Bansal-Yaron (2004) economy. Take $\kappa_{1,c}$ and the intercept of the SDF as known scalars.

\solution  Under No Arbitrage,
\begin{equation}
		P_t = \E_t\left[M_{t+1}\left(P_{t+1}+ D_{t+1}\right)\right],
\end{equation}
which is equivalent to 
\begin{equation}
	\frac{P_t}{D_t} = \E_t\left[M_{t+1}\left(\frac{P_{t+1}+D_{t+1}}{D_{t+1}}\right)\frac{D_{t+1}}{D_t}\right] = \E_t\left[M_{t+1}\left(1 + \frac{P_{t+1}}{D_{t+1}}\right)\frac{D_{t+1}}{D_t}\right],
\end{equation}
i.e.
\begin{equation}\label{eq:additional_ex1_eq1}
	\e{pd_t} = \E_t\left[\e{m_{t+1} + \kappa_{0,d} + \kappa_{1,d} pd_{t+1} + \Delta d_{t+1}}\right],
\end{equation}
because
$$
	1 + \frac{P_{t+1}}{D_{t+1}} = \e{\log\left(1 + \e{pd_{t+1}}\right)},
$$
and
$$
	\log\left(1 + \e{pd_{t+1}}\right) \approx \log\left(1+\e{\pdbar}\right) + \frac{\e{\pdbar}}{1+\e{\pdbar}}\left(pd_{t+1}-\pdbar\right) = \kappa_{0,d} + \kappa_{1,d}pd_{t+1},
$$
with 
\begin{equation}
	\kappa_{1,d} = \frac{\e{\pdbar}}{1+\e{\pdbar}}, \quad\quad \kappa_{0,d} = \log\left(1+\e{\pdbar}\right) - \kappa_{1,d} \pdbar.
\end{equation}
As we usually do, let's conjecture that $pd_{t} = \pdbar + b_d x_t$. Therefore, equation (\ref{eq:additional_ex1_eq1}) becomes
$$
	\begin{aligned}
		\e{\pdbar + b_d x_t} = \E_t\left[\e{m_{t+1} + \kappa_{0,d} + \kappa_{1,d}\left(\pdbar + b_d x_t\right) + \lambda x_t + \varepsilon_{t+1}^d}\right].
	\end{aligned}
$$
Hence, by using our expression for the stochastic discount factor in (\ref{eq:sdf}),
\begin{equation}\label{eq:additional_ex1_eq2}
	\begin{aligned}
		\e{\pdbar + b_d x_t} &= \E_t\left[\e{\bar{m} - \frac{1}{\psi}x_t + \frac{\frac{1}{\psi}-\gamma}{1-\rho\kappa_{1,c}}\kappa_{1,c}\varepsilon_{t+1}^x - \gamma\varepsilon_{t+1}^c+ \kappa_{0,d} + \kappa_{1,d}\left(\pdbar + b_d x_t\right) + \lambda x_t + \varepsilon_{t+1}^d}\right] \\
		\e{\pdbar -\kappa_{0,d} - \kappa_{1,d} \pdbar}\e{b_c x_t} &= \e{\bar{m} + \left[\kappa_{1,d}b_d -\frac{1}{\psi}+ \lambda\right] x_t}\E_t\left[\e{\frac{\frac{1}{\psi}-\gamma}{1-\kappa_{1,c}\rho}\kappa_{1,c}\varepsilon_{t+1}^x -\gamma\varepsilon_{t+1}^c + \varepsilon_{t+1}^d} \right].
	\end{aligned}
\end{equation}
Now note that
\begin{equation}
	\pdbar - \kappa_{0,d} - \kappa_{1,d} \pdbar = \pdbar - \log(1+\e{\pdbar}) + \kappa_{1,d}\pdbar - \kappa_{1,d}\pdbar = \pdbar  - \log(1+\e{\pdbar}),
\end{equation}
and therefore
$$
	\e{\pdbar -\kappa_{0,d} - \kappa_{1,d} \pdbar} = \frac{\e{\pdbar}}{1+\e{\pdbar}} = \kappa_{1,d}.
$$
Hence by also assuming that $x_t \approx \E[x_t] = 0$, (\ref{eq:additional_ex1_eq2}) becomes
$$
	\kappa_{1,d} = \e{\bar{m} + \frac{1}{2}\left[\frac{\ies-\gamma}{1-\kappa_{1,c}\rho}\right]^2\kappa_{1,x}^2\sigma_x^2 +\gamma^2\sigma_c^2 + \sigma_d^2}  .
$$
With our expression for $\bar{m}$ given in (\ref{eq:mbar}), we finally obtain\footnote{Remember that $\zeta= \frac{1}{\theta}$ where $\theta = \frac{1-\gamma}{\alpha}$ as in Bansal and Yaron (2004).}:
\begin{equation}
		\kappa_{1,d} = \e{\zeta\log\delta -\gamma\mu + \half\left[\frac{\ies-\gamma}{1-\kappa_{1,c}\rho}\right]^2\kappa_{1,c}^2\sigma_x^2 +\frac{\gamma^2}{2}\sigma_c^2 + \half\sigma_d^2} .
\end{equation}

